cava/monad-examples/AdderTree.v
@@ -81,7 +81,7 @@ Local Open Scope nat_scope.
 Definition adder_tree_Interface name nrInputs bitSize
   := mkCircuitInterface name
      (One ("inputs", BitVec [nrInputs; bitSize]))
-     (One ("sum", BitVec [bitSize + nrInputs - 1]))
+     (One ("sum", BitVec [bitSize + Nat.log2_up nrInputs]))
      [].
 
 (* Create netlist and test-bench for a 4-input adder tree. *)
